Wavelet/Simulation/Tail.lean
@@ -6,63 +6,44 @@ import Wavelet.Dataflow
 import Wavelet.Compile
 import Wavelet.Lemmas
 
-import Wavelet.Simulation.Relation
+import Wavelet.Simulation.Invariants
 import Wavelet.Simulation.Lemmas
 import Wavelet.Simulation.Ret
 
 namespace Wavelet.Simulation.Tail
 
 open Wavelet.Op Wavelet.Seq Wavelet.Dataflow Wavelet.Compile
-open Relation Lemmas Ret
-
-universe u
-variable (Op : Type u) (χ : Type u) (V S)
-variable [instArity : Arity Op] [DecidableEq χ] [instInterp : Interp Op V S]
+open Invariants Lemmas Ret
 
 /-- Values pushed to output channels in the case of a tail call. -/
-private def exprOutputVals
-  (tailArgs : Vector V m)
-  : Vector V (n + (m + 1)) :=
+def tailArgsToExprOutputs
+  [Arity Op] [instInterp : Interp Op V S]
+  (tailArgs : Vector V m) : Vector V (n + (m + 1)) :=
   Vector.replicate n (Interp.junkVal Op S : V) ++
   tailArgs.push
   (Interp.fromBool Op S true)
 
-set_option maxHeartbeats 1000000
-
 /-- Fires `forwardc` and `sink` to get an intermediate state. -/
 theorem sim_step_tail_forwardc_sink
-  (hnz : m > 0 ∧ n > 0)
+  [Arity Op] [instInterp : Interp Op V S] [DecidableEq χ]
   {ec : Seq.Config Op χ V S m n}
   {pc : Dataflow.Config Op (ChanName χ) V S m n}
-  (hsim : SimR _ _ _ _ hnz ec pc)
+  {hnz : m > 0 ∧ n > 0}
+  (hsim : SimRel hnz ec pc)
   (hexpr : ec.expr = .cont (.tail vars))
   (hvars : VarMap.getVars χ V vars ec.vars = some tailArgs)
   (hvars_nodup : vars.toList.Nodup) :
   Dataflow.Config.StepPlus Op (ChanName χ) V S pc
   { proc := pc.proc,
-    chans := intermChans _ _ _ _ ec pc vars
-      (exprOutputVals Op V S tailArgs)
+    chans := intermChans ec pc vars
+      (tailArgsToExprOutputs (instInterp := instInterp) tailArgs)
       ec.pathConds
     state := pc.state }
 := by
   have ⟨
-    heq_state,
-    hlive_vars,
-    hdefined_vars_no_dup,
-    hdefined_vars,
-    hpath_conds_order,
-    hpath_conds_nodup,
-    hmerges,
-    hwf_fn,
-    ⟨
-      rest, carryInLoop, ctxLeft, ctxCurrent, ctxRight,
-      hatoms,
-      hcomp_fn,
-      hrest,
-      hret,
-      hcont,
-    ⟩,
-  ⟩ := hsim
+    rest, carryInLoop, ctxLeft, ctxCurrent, ctxRight,
+    hatoms, hcomp_fn, hrest, hret, hcont,
+  ⟩ := hsim.has_compiled_procs
   have ⟨hcarryInLoop, hwf_expr, hcurrent⟩ := hcont _ hexpr
   simp [compileExpr] at hcurrent
   -- Some abbreviations
@@ -87,8 +68,8 @@ theorem sim_step_tail_forwardc_sink
       apply List.Nodup.map _ hvars_nodup
       simp [Function.Injective, compileExpr.varName])
     (by
-      simp [← hvar_names, hlive_vars, compileExpr.varNames,
-        compileExpr.varName, SimR.varsToChans]
+      simp [← hvar_names, hsim.vars_to_chans, compileExpr.varNames,
+        compileExpr.varName, varsToChans]
       have := Vector.mapM_some_implies_all_some hvars
       intros v hmem_v
       have ⟨val, _, hval⟩ := this v hmem_v
@@ -102,8 +83,14 @@ theorem sim_step_tail_forwardc_sink
     · simp [← hvar_names, compileExpr.varNames, compileExpr.varName,
         Vector.toList_map, VarMap.getVar]
       apply List.mapM_some_iff_forall₂.mp (Vector.mapM_toList hvars)
-    · simp [Relator.RightUnique, VarMap.getVar]
-      grind
+    · simp only [Relator.RightUnique]
+      intros a b c hb hc
+      have ⟨_, hb₁, hb₂⟩ := hb
+      have ⟨_, hc₁, hc₂⟩ := hc
+      simp [hb₁] at hc₁
+      subst hc₁
+      simp [hb₂] at hc₂
+      exact hc₂
   replace heq_ret_vals := heq_ret_vals.symm
   subst heq_ret_vals
   have hmem_forwardc :
@@ -121,7 +108,7 @@ theorem sim_step_tail_forwardc_sink
   · intros name hmem_name
     simp at hmem_name
     simp [hchans₁, ← hvar_names, compileExpr.varNames,
-      compileExpr.varName, hlive_vars, SimR.varsToChans]
+      compileExpr.varName, hsim.vars_to_chans, varsToChans]
     simp [compileExpr.exprOutputs'] at hmem_name
     rcases hmem_name with ⟨_, _, h⟩ | ⟨_, _, h⟩ | h
     · simp [← h]
@@ -135,14 +122,14 @@ theorem sim_step_tail_forwardc_sink
     (map := pc₁.chans)
     (names := compileExpr.allVarsExcept χ ec.definedVars vars.toList ec.pathConds)
     (λ name val => True)
-    (allVarsExcept_nodup hdefined_vars_no_dup)
+    (allVarsExcept_nodup hsim.defined_vars_nodup)
     (by
       simp
       intros name hname
       have ⟨var, hvar, hmem_var, hnot_mem_var⟩ := mem_allVarsExcept hname
       simp [hvar, hpc₁]
-      simp [hlive_vars, SimR.varsToChans]
-      have ⟨val, h⟩ := (hdefined_vars var).mp hmem_var
+      simp [hsim.vars_to_chans, varsToChans]
+      have ⟨val, h⟩ := hsim.defined_vars_to_get_var hmem_var
       exists val
       simp at hnot_mem_var
       simp [h, ← hvar_names, compileExpr.varNames, compileExpr.varName, hnot_mem_var])
@@ -162,7 +149,7 @@ theorem sim_step_tail_forwardc_sink
   · have ⟨var, hvar, hmem_var, hnot_mem_var⟩ := mem_allVarsExcept h₁
     simp [hvar]
   · split <;> rename_i h₂
-    · simp [exprOutputs'_finIdxOf?_some_to_exprOutputs h₂, ← hjunk, ← htrue, exprOutputVals]
+    · simp [exprOutputs'_finIdxOf?_some_to_exprOutputs h₂, ← hjunk, ← htrue, tailArgsToExprOutputs]
       -- Rearrange positions of tail arguments and return values
       rename_i i
       split_ifs <;> rename_i h₃
@@ -182,7 +169,7 @@ theorem sim_step_tail_forwardc_sink
       simp [this, ← hvar_names]
       split <;> rename_i h₃
       · rfl
-      · simp [hlive_vars, SimR.varsToChans]
+      · simp [hsim.vars_to_chans, varsToChans]
         cases name with
         | var var' pathConds' =>
           simp
@@ -190,43 +177,325 @@ theorem sim_step_tail_forwardc_sink
           simp [h, compileExpr.varNames, compileExpr.varName] at h₃
           simp [compileExpr.allVarsExcept, List.toVector] at h₁
           split <;> rename_i h₄
-          · replace h₄ := (hdefined_vars var').mpr ⟨_, h₄⟩
+          · replace h₄ := hsim.get_var_to_defined_vars ⟨_, h₄⟩
             have := h₁ (List.mem_to_mem_removeAll h₄ (by simp [h₃]))
             simp [h] at this
           · rfl
         | merge_cond condName => rfl
         | _ => simp [hexpr]
 
+set_option maxHeartbeats 300000
+
+/-- Fires relevant operators on the dataflow side. -/
+theorem sim_step_tail_exec_dataflow
+  [Arity Op] [instInterp : Interp Op V S] [DecidableEq χ]
+  {ec ec' : Seq.Config Op χ V S m n}
+  {pc : Dataflow.Config Op (ChanName χ) V S m n}
+  {hnz : m > 0 ∧ n > 0}
+  (hsim : SimRel hnz ec pc)
+  (hstep : Config.Step Op χ V S ec ec')
+  (hexpr : ec.expr = .cont (.tail vars)) :
+  Dataflow.Config.StepPlus Op (ChanName χ) V S pc {
+    proc := pc.proc,
+    chans := varsToChans ec',
+    state := pc.state,
+  }
+:= by
+  have ⟨
+    rest, carryInLoop, ctxLeft, ctxCurrent, ctxRight,
+    hatoms, hcomp_fn, hrest, hret, hcont,
+  ⟩ := hsim.has_compiled_procs
+  have ⟨hcarryInLoop, hwf_expr, hcurrent⟩ := hcont _ hexpr
+  cases hstep with
+  | step_br hexpr' | step_ret hexpr' | step_op hexpr' =>
+    simp [hexpr] at hexpr'
+  | step_tail hexpr' hvars =>
+  rename_i tailArgs vars'
+  simp [hexpr] at hexpr'
+  subst hexpr'
+  cases hwf_expr with | wf_tail hvars_nodup =>
+  -- Step 1: Fire `forwardc` and `sink`
+  have hsteps₁ := sim_step_tail_forwardc_sink hsim hexpr hvars hvars_nodup
+  -- Step 2: Fire final merges
+  have hsteps₂ := sim_step_merges ec pc
+    hsim.has_merges (by simp)
+    hsim.path_conds_nodup hsteps₁
+  -- Step 3: Fire the `fork` in `compileFn`.
+  simp [compileFn, compileFn.resultSteers] at hcomp_fn
+  have ⟨chans₁, hpop_tail_cond, hchans₁⟩ := pop_val_singleton _ _
+    (map := intermChans ec pc vars
+      (tailArgsToExprOutputs (instInterp := instInterp) tailArgs)
+      [])
+    (name := .tail_cond [])
+    (val := instInterp.fromBool true)
+    (by simp [intermChans, exprOutputs_finIdxOf?_tail_cond, tailArgsToExprOutputs])
+  have hmem_fork :
+    .fork (ChanName.tail_cond [])
+      #v[.tail_cond_carry, .tail_cond_steer_dests, .tail_cond_steer_tail_args]
+    ∈ pc.proc.atoms
+  := by simp [hatoms, ← hcomp_fn]
+  have hsteps₃ : Dataflow.Config.StepPlus _ _ _ _ pc _
+    := Relation.TransGen.tail hsteps₂
+      (Dataflow.Config.Step.step_fork hmem_fork hpop_tail_cond)
+  -- Simplify pushes
+  rw [push_vals_empty] at hsteps₃
+  rotate_left
+  · simp
+  · simp [hchans₁, intermChans]
+  simp at hsteps₃
+  replace ⟨pc₁, hpc₁, hsteps₃⟩ := exists_eq_left.mpr hsteps₃
+  -- Step 4: Fire the first `steer` in `compileFn` for return values.
+  have ⟨chans₂, hpop_tail_cond_steer_dests, hchans₂⟩ := pop_val_singleton _ _
+    (map := pc₁.chans)
+    (name := .tail_cond_steer_dests)
+    (val := instInterp.fromBool true)
+    (by simp [hpc₁, List.finIdxOf?, List.findFinIdx?, List.findFinIdx?.go])
+  have ⟨chans₃, retVals, hpop_ret_vals, hchans₃, hret_vals⟩ :=
+    pop_vals_singleton _ _
+    (map := chans₂)
+    (names := (Vector.range n).map (.dest · []))
+    (λ name val => True)
+    (by
+      simp [Vector.toList_map, Vector.toList_range]
+      apply List.Nodup.map _ List.nodup_range
+      simp [Function.Injective])
+    (by
+      intros name hname
+      simp at hname
+      replace ⟨i, h₂, hname⟩ := hname
+      simp [← hname, hchans₂, hpc₁, hchans₁, intermChans,
+        List.finIdxOf?, List.findFinIdx?, List.findFinIdx?.go,
+        exprOutputs_finIdxOf?_dest h₂, h₂, tailArgsToExprOutputs])
+  have hmem_steer_dests :
+    .steer false
+      .tail_cond_steer_dests
+      ((Vector.range n).map (.dest · []))
+      ((Vector.range n).map .final_dest)
+    ∈ pc₁.proc.atoms
+  := by simp [hpc₁, hatoms, ← hcomp_fn]
+  have hsteps₄ : Dataflow.Config.StepPlus _ _ _ _ pc _
+    := Relation.TransGen.tail hsteps₃
+      (Dataflow.Config.Step.step_steer
+        hmem_steer_dests
+        hpop_tail_cond_steer_dests
+        hpop_ret_vals
+        (instInterp.unique_fromBool_toBool _))
+  -- Simplify pushes
+  rw [push_vals_empty] at hsteps₄
+  rotate_left
+  · simp [Vector.toList_map, Vector.toList_range]
+    apply List.Nodup.map _ List.nodup_range
+    simp [Function.Injective]
+  · simp [hchans₃, hchans₂, hpc₁,
+      List.finIdxOf?, List.findFinIdx?, List.findFinIdx?.go,
+      hchans₁, intermChans]
+  simp at hsteps₄
+  replace ⟨pc₂, hpc₂, hsteps₄⟩ := exists_eq_left.mpr hsteps₄
+  -- Step 5: Fire the second `steer` in `compileFn` for tail call args.
+  have ⟨chans₄, hpop_tail_cond_steer_tail_args, hchans₄⟩ := pop_val_singleton _ _
+    (map := pc₂.chans)
+    (name := .tail_cond_steer_tail_args)
+    (val := instInterp.fromBool true)
+    (by
+      simp [hpc₂, hchans₃, hchans₂, hpc₁,
+        List.finIdxOf?, List.findFinIdx?, List.findFinIdx?.go])
+  have ⟨chans₅, tailArgVals, hpop_tail_arg_vals, hchans₅, htail_arg_vals⟩ :=
+    pop_vals_singleton _ _
+    (map := chans₄)
+    (names := (Vector.range m).map (.tail_arg · []))
+    (λ name val =>
+      match name with
+      | .tail_arg i _ => ∃ (h : i < m), val = tailArgs[i]
+      | _ => False)
+    (by
+      simp [Vector.toList_map, Vector.toList_range]
+      apply List.Nodup.map _ List.nodup_range
+      simp [Function.Injective])
+    (by
+      simp
+      intros i hi
+      simp [hchans₄, hpc₂, hchans₃, hchans₂, hpc₁,
+        List.finIdxOf?, List.findFinIdx?, List.findFinIdx?.go,
+        hchans₁, intermChans, tailArgsToExprOutputs,
+        exprOutputs_finIdxOf?_tail_args hi, hi])
+  have : tailArgs = tailArgVals := by
+    symm
+    apply Vector.toList_inj.mp
+    apply List.right_unique_forall₂' _ htail_arg_vals
+    · apply List.forall₂_iff_get.mpr
+      simp [Vector.toList_map, Vector.toList_range]
+    · simp [Relator.RightUnique]
+      intros a b c hb hc
+      split at hb <;> simp at hc
+      replace ⟨_, hb⟩ := hb
+      replace ⟨_, hc⟩ := hc
+      simp [hc, hb]
+  subst this
+  have hmem_steer_tail_args :
+    .steer true
+      .tail_cond_steer_tail_args
+      ((Vector.range m).map (.tail_arg · []))
+      ((Vector.range m).map .final_tail_arg)
+    ∈ pc₂.proc.atoms
+  := by simp [hpc₂, hpc₁, hatoms, ← hcomp_fn]
+  have hsteps₅ : Dataflow.Config.StepPlus _ _ _ _ pc _
+    := Relation.TransGen.tail hsteps₄
+      (Dataflow.Config.Step.step_steer
+        hmem_steer_tail_args
+        hpop_tail_cond_steer_tail_args
+        hpop_tail_arg_vals
+        (instInterp.unique_fromBool_toBool _))
+  rw [push_vals_empty] at hsteps₅
+  rotate_left
+  · simp [Vector.toList_map, Vector.toList_range]
+    apply List.Nodup.map _ List.nodup_range
+    simp [Function.Injective]
+  · simp [hchans₅, hchans₄, hpc₂, hchans₃, hchans₂, hpc₁,
+      List.finIdxOf?, List.findFinIdx?, List.findFinIdx?.go,
+      hchans₁, intermChans]
+  simp at hsteps₅
+  replace ⟨pc₃, hpc₃, hsteps₅⟩ := exists_eq_left.mpr hsteps₅
+  -- Step 6: Fire the first `carry` in `compileFn`.
+  have ⟨chans₆, hpop_tail_cond_steer_tail_args, hchans₆⟩ := pop_val_singleton _ _
+    (map := pc₃.chans)
+    (name := .tail_cond_carry)
+    (val := instInterp.fromBool true)
+    (by simp [hpc₃, hchans₅, hchans₄, hpc₂, hchans₃, hchans₂, hpc₁,
+      List.finIdxOf?, List.findFinIdx?, List.findFinIdx?.go])
+  have ⟨chans₇, tailArgs', hpop_final_tail_args, hchans₇, hfinal_tail_args⟩ :=
+    pop_vals_singleton _ _
+    (map := chans₆)
+    (names := (Vector.range m).map .final_tail_arg)
+    (λ name val =>
+      match name with
+      | .final_tail_arg i => ∃ (h : i < m), val = tailArgs[i]
+      | _ => False)
+    (by
+      simp [Vector.toList_map, Vector.toList_range]
+      apply List.Nodup.map _ List.nodup_range
+      simp [Function.Injective])
+    (by
+      simp
+      intros i hi
+      simp [hchans₆, hpc₃]
+      split <;> rename_i h₁
+      · simp at h₁
+        simp
+        exists hi
+        congr 1
+        omega
+      · have := Option.eq_none_iff_forall_ne_some.mpr h₁
+        simp at this
+        omega)
+  have : tailArgs = tailArgs' := by
+    symm
+    apply Vector.toList_inj.mp
+    apply List.right_unique_forall₂' _ hfinal_tail_args
+    · simp [Vector.toList_map, Vector.toList_range]
+      apply List.forall₂_iff_get.mpr
+      simp
+    · simp [Relator.RightUnique]
+      intros a b c hb hc
+      split at hb <;> simp at hc
+      replace ⟨_, hb⟩ := hb
+      replace ⟨_, hc⟩ := hc
+      simp [hc, hb]
+  subst this
+  have hmem_carry :
+    pc₃.proc.atoms = [] ++ [compileFn.initCarry _ _ _ ec.fn carryInLoop] ++ rest
+  := by simp [hpc₃, hpc₂, hpc₁, hatoms]
+  simp only [compileFn.initCarry, hcarryInLoop] at hmem_carry
+  have hsteps₆ : Dataflow.Config.StepPlus _ _ _ _ pc _
+    := Relation.TransGen.tail hsteps₅
+      (Dataflow.Config.Step.step_carry_true
+        hmem_carry
+        hpop_tail_cond_steer_tail_args
+        (instInterp.unique_fromBool_toBool _)
+        hpop_final_tail_args)
+  -- Simplify pushes
+  rw [push_vals_empty] at hsteps₆
+  rotate_left
+  · simp [Vector.toList_map]
+    apply List.Nodup.map _ hsim.wf_fn.1
+    simp [Function.Injective]
+  · intros name hname
+    simp at hname
+    have ⟨var, hmem_var, hname⟩ := hname
+    simp [← hname, hchans₇, hchans₆, hpc₃, hchans₅, hchans₄, hpc₂,
+      hchans₃, hchans₂, hpc₁,
+      List.finIdxOf?, List.findFinIdx?, List.findFinIdx?.go,
+      hchans₁, intermChans]
+  simp at hsteps₆
+  replace ⟨pc', hpc', hsteps₆⟩ := exists_eq_left.mpr hsteps₆
+  apply step_plus_eq _ _ _ _ hsteps₆
+  simp [hpc', hpc₃, hpc₂, hpc₁,
+    hchans₇, hchans₆, hchans₅, hchans₄, hchans₃, hchans₂, hchans₁,
+    List.finIdxOf?, List.findFinIdx?, List.findFinIdx?.go, intermChans]
+  -- Prove that the final channel maps match
+  funext name
+  simp [varsToChans, Seq.Config.init]
+  cases name with
+  | var v pathConds =>
+    simp
+    if h₁ : pathConds = [] then
+      simp [h₁]
+      split <;> rename_i h₂
+      · rename_i i
+        simp at h₂
+        simp [Vector.get] at h₂
+        simp [← h₂.1]
+        simp [var_map_fromList_get_vars_index hsim.wf_fn.1]
+      · have := Option.eq_none_iff_forall_ne_some.mpr h₂
+        simp at this
+        simp
+        split <;> rename_i h₃
+        · have h₄ := var_map_fromList_get_vars.mpr ⟨_, h₃⟩
+          exact False.elim (this h₄)
+        · rfl
+    else
+      simp [h₁]
+  | dest =>
+    simp
+    intros h₁
+    simp [exprOutputs_finIdxOf?_no_match_dest h₁]
+  | tail_arg =>
+    simp
+    intros h₁
+    simp [exprOutputs_finIdxOf?_no_match_tail_args h₁]
+  | tail_cond =>
+    simp
+    intros h₁
+    simp [exprOutputs_finIdxOf?_no_match_tail_cond h₁]
+  | final_tail_arg =>
+    simp
+    split <;> rename_i h₁
+    · simp at h₁
+      omega
+    · simp
+  | input | switch_cond | merge_cond
+  | tail_cond_carry | tail_cond_steer_dests | tail_cond_steer_tail_args
+  | final_dest =>
+    simp
+
 /-- TODO: these theorems are similar to `sim_step_ret`,
 figure out a way to share these proofs. -/
 theorem sim_step_tail
-  (hnz : m > 0 ∧ n > 0)
-  (ec ec' : Seq.Config Op χ V S m n)
-  (pc : Dataflow.Config Op (ChanName χ) V S m n)
-  (hsim : SimR _ _ _ _ hnz ec pc)
+  [Arity Op] [instInterp : Interp Op V S] [DecidableEq χ]
+  {ec ec' : Seq.Config Op χ V S m n}
+  {pc : Dataflow.Config Op (ChanName χ) V S m n}
+  {hnz : m > 0 ∧ n > 0}
+  (hsim : SimRel hnz ec pc)
   (hstep : Config.Step Op χ V S ec ec')
   (hexpr : ec.expr = .cont (.tail vars)) :
   ∃ pc',
     Config.StepPlus Op (ChanName χ) V S pc pc' ∧
-    SimR _ _ _ _ hnz ec' pc' := by
+    SimRel hnz ec' pc' := by
+  have hsteps := sim_step_tail_exec_dataflow hsim hstep hexpr
+  replace ⟨pc', hpc', hsteps⟩ := exists_eq_left.mpr hsteps
   have ⟨
-    heq_state,
-    hlive_vars,
-    hdefined_vars_no_dup,
-    hdefined_vars,
-    hpath_conds_order,
-    hpath_conds_nodup,
-    hmerges,
-    hwf_fn,
-    ⟨
-      rest, carryInLoop, ctxLeft, ctxCurrent, ctxRight,
-      hatoms,
-      hcomp_fn,
-      hrest,
-      hret,
-      hcont,
-    ⟩,
-  ⟩ := hsim
+    rest, carryInLoop, ctxLeft, ctxCurrent, ctxRight,
+    hatoms, hcomp_fn, hrest, hret, hcont,
+  ⟩ := hsim.has_compiled_procs
   have ⟨hcarryInLoop, hwf_expr, hcurrent⟩ := hcont _ hexpr
   cases hstep with
   | step_br hexpr' | step_ret hexpr' | step_op hexpr' =>
@@ -236,309 +505,30 @@ theorem sim_step_tail
     simp [hexpr] at hexpr'
     subst hexpr'
     cases hwf_expr with | wf_tail hvars_nodup =>
-    have hsteps₁ :=
-      sim_step_tail_forwardc_sink _ _ _ _ hnz hsim hexpr hvars hvars_nodup
-    have hsteps₂ := sim_step_merges _ _ _ _ ec pc
-      hmerges (by simp)
-      hpath_conds_nodup hsteps₁
-    -- Step 4: Fire the `fork` in `compileFn`.
-    simp only [compileFn, compileFn.resultSteers] at hcomp_fn
-    have ⟨chans₁, hpop_tail_cond, hchans₁⟩ := pop_val_singleton _ _
-      (map := intermChans _ _ _ _ ec pc vars
-        (exprOutputVals Op V S tailArgs)
-        [])
-      (name := .tail_cond [])
-      (val := instInterp.fromBool true)
-      (by simp [intermChans, exprOutputs_finIdxOf?_tail_cond, exprOutputVals])
-    have hmem_fork :
-      .fork (ChanName.tail_cond [])
-        #v[.tail_cond_carry, .tail_cond_steer_dests, .tail_cond_steer_tail_args]
-      ∈ pc.proc.atoms
-    := by grind
-    have hsteps₃ : Dataflow.Config.StepPlus _ _ _ _ pc _
-      := Relation.TransGen.tail hsteps₂
-        (Dataflow.Config.Step.step_fork hmem_fork hpop_tail_cond)
-    -- Simplify pushes
-    rw [push_vals_empty] at hsteps₃
-    rotate_left
-    · simp
-    · simp [hchans₁, intermChans]
-    simp at hsteps₃
-    replace ⟨pc₁, hpc₁, hsteps₃⟩ := exists_eq_left.mpr hsteps₃
-    -- Step 5: Fire the first `steer` in `compileFn` for return values.
-    have ⟨chans₂, hpop_tail_cond_steer_dests, hchans₂⟩ := pop_val_singleton _ _
-      (map := pc₁.chans)
-      (name := .tail_cond_steer_dests)
-      (val := instInterp.fromBool true)
-      (by simp [hpc₁, List.finIdxOf?, List.findFinIdx?, List.findFinIdx?.go])
-    have ⟨chans₃, retVals, hpop_ret_vals, hchans₃, hret_vals⟩ :=
-      pop_vals_singleton _ _
-      (map := chans₂)
-      (names := (Vector.range n).map (.dest · []))
-      (λ name val => True)
-      (by
-        simp [Vector.toList_map, Vector.toList_range]
-        apply List.Nodup.map _ List.nodup_range
-        simp [Function.Injective])
-      (by
-        intros name hname
-        simp at hname
-        replace ⟨i, h₂, hname⟩ := hname
-        simp [← hname, hchans₂, hpc₁, hchans₁, intermChans,
-          List.finIdxOf?, List.findFinIdx?, List.findFinIdx?.go,
-          exprOutputs_finIdxOf?_dest h₂, h₂, exprOutputVals])
-    have hmem_steer_dests :
-      .steer false
-        .tail_cond_steer_dests
-        ((Vector.range n).map (.dest · []))
-        ((Vector.range n).map .final_dest)
-      ∈ pc₁.proc.atoms
-    := by grind
-    have hsteps₄ : Dataflow.Config.StepPlus _ _ _ _ pc _
-      := Relation.TransGen.tail hsteps₃
-        (Dataflow.Config.Step.step_steer
-          hmem_steer_dests
-          hpop_tail_cond_steer_dests
-          hpop_ret_vals
-          (instInterp.unique_fromBool_toBool _))
-    -- Simplify pushes
-    rw [push_vals_empty] at hsteps₄
-    rotate_left
-    · simp [Vector.toList_map, Vector.toList_range]
-      apply List.Nodup.map _ List.nodup_range
-      simp [Function.Injective]
-    · simp [hchans₃, hchans₂, hpc₁,
-        List.finIdxOf?, List.findFinIdx?, List.findFinIdx?.go,
-        hchans₁, intermChans]
-    simp at hsteps₄
-    replace ⟨pc₂, hpc₂, hsteps₄⟩ := exists_eq_left.mpr hsteps₄
-    -- Step 6: Fire the second `steer` in `compileFn` for tail call args.
-    have ⟨chans₄, hpop_tail_cond_steer_tail_args, hchans₄⟩ := pop_val_singleton _ _
-      (map := pc₂.chans)
-      (name := .tail_cond_steer_tail_args)
-      (val := instInterp.fromBool true)
-      (by
-        simp [hpc₂, hchans₃, hchans₂, hpc₁,
-          List.finIdxOf?, List.findFinIdx?, List.findFinIdx?.go])
-    have ⟨chans₅, tailArgVals, hpop_tail_arg_vals, hchans₅, htail_arg_vals⟩ :=
-      pop_vals_singleton _ _
-      (map := chans₄)
-      (names := (Vector.range m).map (.tail_arg · []))
-      (λ name val =>
-        match name with
-        | .tail_arg i _ => ∃ (h : i < m), val = tailArgs[i]
-        | _ => False)
-      (by
-        simp [Vector.toList_map, Vector.toList_range]
-        apply List.Nodup.map _ List.nodup_range
-        simp [Function.Injective])
-      (by
-        simp
-        intros i hi
-        simp [hchans₄, hpc₂, hchans₃, hchans₂, hpc₁,
-          List.finIdxOf?, List.findFinIdx?, List.findFinIdx?.go,
-          hchans₁, intermChans, exprOutputVals,
-          exprOutputs_finIdxOf?_tail_args hi, hi])
-    have : tailArgs = tailArgVals := by
-      symm
-      apply Vector.toList_inj.mp
-      apply List.right_unique_forall₂' _ htail_arg_vals
-      · apply List.forall₂_iff_get.mpr
-        simp [Vector.toList_map, Vector.toList_range]
-      · simp [Relator.RightUnique]
-        intros a b c hb hc
-        split at hb <;> simp at hc
-        replace ⟨_, hb⟩ := hb
-        replace ⟨_, hc⟩ := hc
-        simp [hc, hb]
-    subst this
-    have hmem_steer_tail_args :
-      .steer true
-        .tail_cond_steer_tail_args
-        ((Vector.range m).map (.tail_arg · []))
-        ((Vector.range m).map .final_tail_arg)
-      ∈ pc₂.proc.atoms
-    := by grind
-    have hsteps₅ : Dataflow.Config.StepPlus _ _ _ _ pc _
-      := Relation.TransGen.tail hsteps₄
-        (Dataflow.Config.Step.step_steer
-          hmem_steer_tail_args
-          hpop_tail_cond_steer_tail_args
-          hpop_tail_arg_vals
-          (instInterp.unique_fromBool_toBool _))
-    rw [push_vals_empty] at hsteps₅
-    rotate_left
-    · simp [Vector.toList_map, Vector.toList_range]
-      apply List.Nodup.map _ List.nodup_range
-      simp [Function.Injective]
-    · simp [hchans₅, hchans₄, hpc₂, hchans₃, hchans₂, hpc₁,
-        List.finIdxOf?, List.findFinIdx?, List.findFinIdx?.go,
-        hchans₁, intermChans]
-    simp at hsteps₅
-    replace ⟨pc₃, hpc₃, hsteps₅⟩ := exists_eq_left.mpr hsteps₅
-    -- Step 7: Fire the first `carry` in `compileFn`.
-    have ⟨chans₆, hpop_tail_cond_steer_tail_args, hchans₆⟩ := pop_val_singleton _ _
-      (map := pc₃.chans)
-      (name := .tail_cond_carry)
-      (val := instInterp.fromBool true)
-      (by simp [hpc₃, hchans₅, hchans₄, hpc₂, hchans₃, hchans₂, hpc₁,
-        List.finIdxOf?, List.findFinIdx?, List.findFinIdx?.go])
-    have ⟨chans₇, tailArgs', hpop_final_tail_args, hchans₇, hfinal_tail_args⟩ :=
-      pop_vals_singleton _ _
-      (map := chans₆)
-      (names := (Vector.range m).map .final_tail_arg)
-      (λ name val =>
-        match name with
-        | .final_tail_arg i => ∃ (h : i < m), val = tailArgs[i]
-        | _ => False)
-      (by
-        simp [Vector.toList_map, Vector.toList_range]
-        apply List.Nodup.map _ List.nodup_range
-        simp [Function.Injective])
-      (by
-        simp
-        intros i hi
-        simp [hchans₆, hpc₃]
-        split <;> rename_i h₁
-        · simp at h₁
-          simp
-          exists hi
-          congr 1
-          omega
-        · have := Option.eq_none_iff_forall_ne_some.mpr h₁
-          simp at this
-          omega)
-    have : tailArgs = tailArgs' := by
-      symm
-      apply Vector.toList_inj.mp
-      apply List.right_unique_forall₂' _ hfinal_tail_args
-      · simp [Vector.toList_map, Vector.toList_range]
-        apply List.forall₂_iff_get.mpr
-        simp
-      · simp [Relator.RightUnique]
-        intros a b c hb hc
-        split at hb <;> simp at hc
-        replace ⟨_, hb⟩ := hb
-        replace ⟨_, hc⟩ := hc
-        simp [hc, hb]
-    subst this
-    have hmem_carry :
-      pc₃.proc.atoms = [] ++ [compileFn.initCarry _ _ _ ec.fn carryInLoop] ++ rest
-    := by simp [hpc₃, hpc₂, hpc₁, hatoms]
-    simp only [compileFn.initCarry, hcarryInLoop] at hmem_carry
-    have hsteps₆ : Dataflow.Config.StepPlus _ _ _ _ pc _
-      := Relation.TransGen.tail hsteps₅
-        (Dataflow.Config.Step.step_carry_true
-          hmem_carry
-          hpop_tail_cond_steer_tail_args
-          (instInterp.unique_fromBool_toBool _)
-          hpop_final_tail_args)
-    -- Simplify pushes
-    rw [push_vals_empty] at hsteps₆
-    rotate_left
-    · simp [Vector.toList_map]
-      apply List.Nodup.map _ hwf_fn.1
-      simp [Function.Injective]
-    · intros name hname
-      simp at hname
-      have ⟨var, hmem_var, hname⟩ := hname
-      simp [← hname, hchans₇, hchans₆, hpc₃, hchans₅, hchans₄, hpc₂,
-        hchans₃, hchans₂, hpc₁,
-        List.finIdxOf?, List.findFinIdx?, List.findFinIdx?.go,
-        hchans₁, intermChans]
-    simp at hsteps₆
-    replace ⟨pc', hpc', hsteps₆⟩ := exists_eq_left.mpr hsteps₆
-    -- Step 8: Prove preservation of invariants.
     exists pc'
     constructor
-    · exact hsteps₆
-    · simp only [Seq.Config.init]
+    · exact hsteps
+    · simp only [Seq.Config.init, hpc']
       and_intros
-      · simp only [heq_state, hpc', hpc₃, hpc₂, hpc₁]
-      · -- varsToChans
-        funext name
-        simp [SimR.varsToChans]
-        cases name with
-        | var v pathConds =>
-          simp [hpc', hchans₇, hchans₆, hpc₃, hchans₅, hchans₄, hpc₂,
-            hchans₃, hchans₂, hpc₁]
-          if h₁ : pathConds = [] then
-            simp [h₁]
-            split <;> rename_i h₂
-            · rename_i i
-              simp at h₂
-              simp [Vector.get] at h₂
-              simp [← h₂.1]
-              simp [var_map_fromList_get_vars_index hwf_fn.1]
-            · have := Option.eq_none_iff_forall_ne_some.mpr h₂
-              simp at this
-              simp [List.finIdxOf?, List.findFinIdx?, List.findFinIdx?.go,
-                hchans₁, intermChans]
-              split <;> rename_i h₃
-              · have h₄ := var_map_fromList_get_vars.mpr ⟨_, h₃⟩
-                exact False.elim (this h₄)
-              · rfl
-          else
-            simp [h₁, List.finIdxOf?, List.findFinIdx?, List.findFinIdx?.go,
-              hchans₁, intermChans]
-        | dest =>
-          simp [hpc', hchans₇, hchans₆, hpc₃, hchans₅, hchans₄, hpc₂,
-            hchans₃, hchans₂, hpc₁,
-            List.finIdxOf?, List.findFinIdx?, List.findFinIdx?.go,
-            hchans₁, intermChans]
-          intros h₁
-          simp [exprOutputs_finIdxOf?_no_match_dest h₁]
-        | tail_arg =>
-          simp [hpc', hchans₇, hchans₆, hpc₃, hchans₅, hchans₄, hpc₂,
-            hchans₃, hchans₂, hpc₁,
-            List.finIdxOf?, List.findFinIdx?, List.findFinIdx?.go,
-            hchans₁, intermChans]
-          intros h₁
-          simp [exprOutputs_finIdxOf?_no_match_tail_args h₁]
-        | tail_cond =>
-          simp [hpc', hchans₇, hchans₆, hpc₃, hchans₅, hchans₄, hpc₂,
-            hchans₃, hchans₂, hpc₁,
-            List.finIdxOf?, List.findFinIdx?, List.findFinIdx?.go,
-            hchans₁, intermChans]
-          intros h₁
-          simp [exprOutputs_finIdxOf?_no_match_tail_cond h₁]
-        | input | switch_cond | merge_cond
-        | tail_cond_carry | tail_cond_steer_dests | tail_cond_steer_tail_args
-        | final_dest =>
-          simp [hpc', hchans₇, hchans₆, hpc₃, hchans₅, hchans₄, hpc₂,
-            hchans₃, hchans₂, hpc₁,
-            List.finIdxOf?, List.findFinIdx?, List.findFinIdx?.go,
-            hchans₁, intermChans]
-        | final_tail_arg =>
-          simp [hpc', hchans₇, hchans₆, hpc₃, hchans₅, hchans₄, hpc₂,
-            hchans₃, hchans₂, hpc₁,
-            List.finIdxOf?, List.findFinIdx?, List.findFinIdx?.go,
-            hchans₁, intermChans]
-          split <;> rename_i h₁
-          · simp at h₁
-            omega
-          · simp
-      · simp [hwf_fn.1]
+      · simp only [hsim.eq_state]
+      · simp
+      · simp [hsim.wf_fn.1]
       · simp []
         intros var
         apply var_map_fromList_get_vars
-      · simp [SimR.OrderedPathConds]
+      · simp [OrderedPathConds]
       · simp
-      · simp [SimR.HasMerges]
-      · exact hwf_fn.1
-      · exact hwf_fn.2
-      · exists rest, true
-        -- ctxLeft
-        exists []
-        -- ctxCurrent
-        exists compileExpr Op χ V S hnz ec.fn.params.toList [] ec.fn.body
-        -- ctxRight
-        exists compileFn.resultSteers Op χ V m n
-        simp [hrest] at hcomp_fn
-        simp [hpc', hpc₃, hpc₂, hpc₁,
-          compileFn.initCarry, compileFn, hatoms,
-          compileFn.initCarry, hcarryInLoop, hrest,
-          hwf_fn.2, compileFn.bodyComp, compileFn.resultSteers,
-          ← hcomp_fn]
+      · simp [HasMerges]
+      · exact hsim.wf_fn.1
+      · exact hsim.wf_fn.2
+      · simp [compileFn.initCarry, HasCompiledProcs]
+        exists rest
+        simp [hatoms, compileFn, compileFn.initCarry, hcarryInLoop]
+        simp [compileFn] at hcomp_fn
+        simp [hcomp_fn]
+        constructor
+        · exists [], compileFn.resultSteers Op χ V m n
+          simp [← hcomp_fn, compileFn.bodyComp]
+        · exact hsim.wf_fn.2
 
 end Wavelet.Simulation.Tail
