Wavelet/Simulation/Br.lean
@@ -9,285 +9,243 @@ import Wavelet.Dataflow
 import Wavelet.Compile
 import Wavelet.Lemmas
 
-import Wavelet.Simulation.Relation
+import Wavelet.Simulation.Invariants
 import Wavelet.Simulation.Lemmas
+
+/-! Simulation in the case of branching. -/
 
 namespace Wavelet.Simulation.Br
 
 open Wavelet.Op Wavelet.Seq Wavelet.Dataflow Wavelet.Compile
-open Relation Lemmas
+open Invariants Lemmas
 
 /-- Helper lemma to run relevant dataflow operators. -/
-theorem sim_step_br_chans
+theorem sim_step_br_exec_dataflow
   [Arity Op] [DecidableEq χ] [instInterp : Interp Op V S]
   {cond left right}
   {ec ec' : Seq.Config Op χ V S m n}
   {pc : Dataflow.Config Op (ChanName χ) V S m n}
-  (hnz : m > 0 ∧ n > 0)
-  (hsim : SimR _ _ _ _ hnz ec pc)
+  {hnz : m > 0 ∧ n > 0}
+  (hsim : SimRel hnz ec pc)
   (hstep : Config.Step Op χ V S ec ec')
   (hbr : ec.expr = .cont (.br cond left right)) :
   Dataflow.Config.StepPlus Op (ChanName χ) V S pc {
     proc := pc.proc,
-    chans := SimR.varsToChans _ _ _ _ ec',
+    chans := varsToChans ec',
     state := pc.state,
   } := by
+  -- Unpack compiled processes
   have ⟨
-    heq_state,
-    hlive_vars,
-    hdefined_vars_no_dup,
-    hdefined_vars,
-    hpath_conds_order,
-    hpath_conds_nodup,
-    hmerges,
-    hwf_fn,
-    ⟨
-      rest, carryInLoop, ctxLeft, ctxCurrent, ctxRight,
-      hatoms,
-      hcomp_fn,
-      hrest,
-      hret,
-      hcont,
-    ⟩,
-  ⟩ := hsim
+    rest, carryInLoop, ctxLeft, ctxCurrent, ctxRight,
+    hatoms, hcomp_fn, hrest, hret, hcont,
+  ⟩ := hsim.has_compiled_procs
   have ⟨hcarryInLoop, hwf_expr, hcurrent⟩ := hcont _ hbr
   simp only [compileExpr] at hcurrent
   -- Deduce some facts from `hstep`
   cases hstep with
-  | step_ret hexpr | step_tail hexpr | step_op hexpr =>
-    simp [hbr] at hexpr
+  | step_ret hexpr | step_tail hexpr | step_op hexpr => simp [hbr] at hexpr
   | step_br hexpr hcond hcondBool =>
-    rename_i condVal condBool _ _ cond'
-    simp only [hbr, ExprResult.cont.injEq, Expr.br.injEq] at hexpr
-    have heq_cond' := hexpr.1; subst heq_cond'
-    have heq_left' := hexpr.2.1; subst heq_left'
-    have heq_right' := hexpr.2.2; subst heq_right'
-    clear hexpr
-    cases hwf_expr with | wf_br hwf_left hwf_right =>
-    -- Some abbreviations
-    generalize hcondName :
-      compileExpr.varName χ ec.pathConds cond = condName
-    simp only [hcondName] at hcurrent
-    simp only [compileExpr.varName] at hcondName
-    generalize hleftConds : (true, condName) :: ec.pathConds = leftConds
-    generalize hrightConds : (false, condName) :: ec.pathConds = rightConds
-    simp only [hleftConds, hrightConds] at hcurrent
-    generalize hleftComp :
-      compileExpr Op χ V S hnz (ec.definedVars.removeAll [cond]) leftConds left = leftComp
-    generalize hrightComp :
-      compileExpr Op χ V S hnz (ec.definedVars.removeAll [cond]) rightConds right = rightComp
-    simp only [hleftComp, hrightComp] at hcurrent
-    -- Step 1: Pop `cond` and fire the first `fork`.
-    have hcondVal : pc.chans condName = [condVal]
-      := by simp [hlive_vars, SimR.varsToChans, hcond, ← hcondName]
-    have ⟨chans₁, hpop_cond, hchans₁⟩ := pop_val_singleton _ _
-      (map := pc.chans)
-      (name := condName)
-      (val := condVal)
-      (by simp [hlive_vars, SimR.varsToChans, hcond, ← hcondName])
-    have hmem_fork :
-      .fork condName #v[.switch_cond condName, .merge_cond condName] ∈ pc.proc.atoms
-      := by simp [hatoms, hrest, ← hcurrent]
-    have hsteps₁ : Dataflow.Config.StepPlus _ _ _ _ pc _
-      := Relation.TransGen.single (Dataflow.Config.Step.step_fork hmem_fork hpop_cond)
-    -- Simplify pushes
-    rw [push_vals_empty] at hsteps₁
-    rotate_left
-    · simp
-    · simp [hchans₁, ← hcondName, hlive_vars, SimR.varsToChans,
-        path_conds_acyclic hpath_conds_order]
-    replace ⟨pc₁, hpc₁, hsteps₁⟩ := exists_eq_left.mpr hsteps₁
-    -- Step 2: Pop `switch_cond` and all live variable, and fire the `switch` operator
-    have ⟨chans₂, hpop_switch_cond, hchans₂⟩ := pop_val_singleton _ _
-      (map := pc₁.chans)
-      (val := condVal)
-      (name := .switch_cond condName)
-      (by simp [hpc₁, List.finIdxOf?, List.findFinIdx?, List.findFinIdx?.go])
-    have ⟨chans₃, allVals, hpop_all_vals, hchans₃, hall_vals⟩ :=
-      pop_vals_singleton _ _
-      (map := chans₂)
-      (names := compileExpr.allVarsExcept χ ec.definedVars [cond] ec.pathConds)
-      (λ name val =>
-        ∃ var,
-          name = .var var ec.pathConds ∧
-          ec.vars.getVar _ _ var = some val)
-      (allVarsExcept_nodup hdefined_vars_no_dup)
-      (by
-        intros name hname
-        have ⟨var, hvar, hmem_var, hnot_mem_var⟩ := mem_allVarsExcept hname
-        simp only [List.mem_cons, List.not_mem_nil, or_false] at hnot_mem_var
-        simp only [List.removeAll, compileExpr.allVarsExcept, Vector.mem_map] at hname
-        have ⟨_, h⟩ := (hdefined_vars var).mp hmem_var
-        simp [h, hchans₁, hchans₂, hpc₁, hvar, hnot_mem_var, ← hcondName, hlive_vars,
-          SimR.varsToChans, List.finIdxOf?, List.findFinIdx?, List.findFinIdx?.go])
-    have hchans₃_no_var {var pathConds} : chans₃ (.var var pathConds) = []
-    := by
-      simp [hchans₃, hchans₂, hchans₁, hpc₁, hlive_vars, ← hcondName,
-        SimR.varsToChans, VarMap.getVar, compileExpr.allVarsExcept, List.toVector,
+  rename_i condVal condBool _ _ cond'
+  simp only [hbr, ExprResult.cont.injEq, Expr.br.injEq] at hexpr
+  have h := hexpr.1; subst h
+  have h := hexpr.2.1; subst h
+  have h := hexpr.2.2; subst h
+  clear hexpr
+  cases hwf_expr with | wf_br hwf_left hwf_right =>
+  -- Some abbreviations
+  generalize hcond_name :
+    compileExpr.varName χ ec.pathConds cond = condName
+  simp only [hcond_name] at hcurrent
+  simp only [compileExpr.varName] at hcond_name
+  generalize hleft_conds : (true, condName) :: ec.pathConds = leftConds
+  generalize hright_conds : (false, condName) :: ec.pathConds = rightConds
+  simp only [hleft_conds, hright_conds] at hcurrent
+  -- Step 1: Pop `cond` and fire the first `fork`.
+  have hcondVal : pc.chans condName = [condVal]
+    := by simp [hsim.vars_to_chans, varsToChans, hcond, ← hcond_name]
+  have ⟨chans₁, hpop_cond, hchans₁⟩ := pop_val_singleton _ _
+    (map := pc.chans)
+    (name := condName)
+    (val := condVal)
+    (by simp [hsim.vars_to_chans, varsToChans, hcond, ← hcond_name])
+  have hmem_fork :
+    .fork condName #v[.switch_cond condName, .merge_cond condName] ∈ pc.proc.atoms
+    := by simp [hatoms, hrest, ← hcurrent]
+  have hsteps₁ : Dataflow.Config.StepPlus _ _ _ _ pc _
+    := Relation.TransGen.single (Dataflow.Config.Step.step_fork hmem_fork hpop_cond)
+  -- Simplify pushes
+  rw [push_vals_empty] at hsteps₁
+  rotate_left
+  · simp
+  · simp [hchans₁, ← hcond_name, hsim.vars_to_chans, varsToChans, hsim.path_conds_acyclic]
+  replace ⟨pc₁, hpc₁, hsteps₁⟩ := exists_eq_left.mpr hsteps₁
+  -- Step 2: Pop `switch_cond` and all live variable, and fire the `switch` operator
+  have ⟨chans₂, hpop_switch_cond, hchans₂⟩ := pop_val_singleton _ _
+    (map := pc₁.chans)
+    (val := condVal)
+    (name := .switch_cond condName)
+    (by simp [hpc₁, List.finIdxOf?, List.findFinIdx?, List.findFinIdx?.go])
+  have ⟨chans₃, allVals, hpop_all_vals, hchans₃, hall_vals⟩ :=
+    pop_vals_singleton _ _
+    (map := chans₂)
+    (names := compileExpr.allVarsExcept χ ec.definedVars [cond] ec.pathConds)
+    (λ name val =>
+      ∃ var,
+        name = .var var ec.pathConds ∧
+        ec.vars.getVar _ _ var = some val)
+    (allVarsExcept_nodup hsim.defined_vars_nodup)
+    (by
+      intros name hname
+      have ⟨var, hvar, hmem_var, hnot_mem_var⟩ := mem_allVarsExcept hname
+      simp only [List.mem_cons, List.not_mem_nil, or_false] at hnot_mem_var
+      simp only [List.removeAll, compileExpr.allVarsExcept, Vector.mem_map] at hname
+      have ⟨_, h⟩ := hsim.defined_vars_to_get_var hmem_var
+      simp [h, hchans₁, hchans₂, hpc₁, hvar, hnot_mem_var, ← hcond_name, hsim.vars_to_chans,
+        varsToChans, List.finIdxOf?, List.findFinIdx?, List.findFinIdx?.go])
+  have hchans₃_no_var {var pathConds} : chans₃ (.var var pathConds) = []
+  := by
+    simp [hchans₃, hchans₂, hchans₁, hpc₁, hsim.vars_to_chans, ← hcond_name,
+      varsToChans, VarMap.getVar, compileExpr.allVarsExcept, List.toVector,
+      List.finIdxOf?, List.findFinIdx?, List.findFinIdx?.go]
+    intros h₁ h₂ h₃
+    split
+    · rename_i h₄
+      have := hsim.get_var_to_defined_vars ⟨_, h₄⟩
+      if h₅ : var = cond then
+        simp [h₂ h₅ h₃]
+      else
+        simp [h₁ (List.mem_filter.mpr ⟨this, by simp [h₅]⟩) h₃.symm]
+    · rfl
+  have hsteps₂ : Dataflow.Config.StepPlus _ _ _ _ pc _
+    := Relation.TransGen.tail hsteps₁
+        (Dataflow.Config.Step.step_switch
+          (by simp [hpc₁, hatoms, hrest, ← hcurrent])
+          hpop_switch_cond
+          hpop_all_vals
+          hcondBool
+          (decider := .switch_cond condName)
+          (inputs := compileExpr.allVarsExcept χ ec.definedVars [cond] ec.pathConds)
+          (outputs₁ := compileExpr.allVarsExcept χ ec.definedVars [cond] leftConds)
+          (outputs₂ := compileExpr.allVarsExcept χ ec.definedVars [cond] rightConds))
+  simp only at hsteps₂
+  -- Simplify pushes
+  rw [push_vals_empty] at hsteps₂
+  rotate_left
+  · split <;> apply allVarsExcept_nodup hsim.defined_vars_nodup
+  · split
+    all_goals
+      intros name hname
+      simp only [compileExpr.allVarsExcept, Vector.mem_map] at hname
+      replace ⟨var, hvar, hname⟩ := hname
+      simp only [List.toVector, Vector.mem_mk, Array.mem_toArray] at hvar
+      simp [hchans₁, hchans₂, hchans₃, hpc₁, ← hname,
+        compileExpr.allVarsExcept, List.toVector,
+        List.finIdxOf?, List.findFinIdx?, List.findFinIdx?.go,
+        hsim.vars_to_chans, varsToChans]
+      intros h₁ _ h₂
+      exact False.elim (h₁ hvar h₂.symm)
+  have :
+    (if condBool = true then
+      compileExpr.allVarsExcept χ ec.definedVars [cond] leftConds
+    else
+      compileExpr.allVarsExcept χ ec.definedVars [cond] rightConds)
+    = compileExpr.allVarsExcept χ ec.definedVars [cond]
+      ((condBool, ChanName.var cond ec.pathConds) :: ec.pathConds)
+  := by
+    simp only [← hleft_conds, ← hright_conds, ← hcond_name]
+    cases condBool <;> simp
+  rw [this] at hsteps₂; clear this
+  apply step_plus_eq _ _ _ _ hsteps₂
+  simp [hpc₁]
+  funext name
+  simp only [varsToChans]
+  cases name with
+  | var v pathConds =>
+    simp
+    if h₁ : v = cond then
+      rw [allVarsExcept_finIdxOf?_none_if_removed (by simp [h₁])]
+      simp [h₁, VarMap.getVar, VarMap.removeVar, hchans₃, hchans₂, hpc₁, hchans₁,
+        hsim.vars_to_chans, varsToChans, ← hcond_name,
         List.finIdxOf?, List.findFinIdx?, List.findFinIdx?.go]
-      intros h₁ h₂ h₃
-      split
-      · rename_i h₄
-        have := (hdefined_vars var).mpr ⟨_, h₄⟩
-        if h₅ : var = cond then
-          simp [h₂ h₅ h₃]
+      intros _ h₂ h₃
+      exact False.elim (h₂ h₃)
+    else
+      if h₂ : v ∈ ec.definedVars then
+        if h₃ : pathConds = (condBool, ChanName.var cond ec.pathConds) :: ec.pathConds then
+          have ⟨i, h₄⟩ := allVarsExcept_finIdxOf?_some (removedVars := [cond])
+            h₂ (by simp [h₁]) h₃
+          simp [h₄]
+          simp [compileExpr.allVarsExcept] at h₄
+          simp [List.toVector] at h₄
+          simp [h₄.1.2, Ne.symm h₁, VarMap.getVar, VarMap.removeVar]
+          have ⟨_, h₅⟩ := hsim.defined_vars_to_get_var h₂
+          simp only [VarMap.getVar] at h₅
+          have := List.forall₂_iff_get.mp hall_vals
+          have := this.2 i (by simp) (by simp)
+          simp [List.toVector, VarMap.getVar, compileExpr.allVarsExcept, h₄.1.1] at this
+          simp [this]
         else
-          simp [h₁ (List.mem_filter.mpr ⟨this, by simp [h₅]⟩) h₃.symm]
-      · rfl
-    have hsteps₂ : Dataflow.Config.StepPlus _ _ _ _ pc _
-      := Relation.TransGen.tail hsteps₁
-          (Dataflow.Config.Step.step_switch
-            (by simp [hpc₁, hatoms, hrest, ← hcurrent])
-            hpop_switch_cond
-            hpop_all_vals
-            hcondBool
-            (decider := .switch_cond condName)
-            (inputs := compileExpr.allVarsExcept χ ec.definedVars [cond] ec.pathConds)
-            (outputs₁ := compileExpr.allVarsExcept χ ec.definedVars [cond] leftConds)
-            (outputs₂ := compileExpr.allVarsExcept χ ec.definedVars [cond] rightConds))
-    simp only at hsteps₂
-    -- Simplify pushes
-    rw [push_vals_empty] at hsteps₂
-    rotate_left
-    · split <;> apply allVarsExcept_nodup hdefined_vars_no_dup
-    · split
-      all_goals
-        intros name hname
-        simp only [compileExpr.allVarsExcept, Vector.mem_map] at hname
-        replace ⟨var, hvar, hname⟩ := hname
-        simp only [List.toVector, Vector.mem_mk, Array.mem_toArray] at hvar
-        simp [hchans₁, hchans₂, hchans₃, hpc₁, ← hname,
-          compileExpr.allVarsExcept, List.toVector,
-          List.finIdxOf?, List.findFinIdx?, List.findFinIdx?.go,
-          hlive_vars, SimR.varsToChans]
-        intros h₁ _ h₂
-        exact False.elim (h₁ hvar h₂.symm)
-    have :
-      (if condBool = true then
-        compileExpr.allVarsExcept χ ec.definedVars [cond] leftConds
+          rw [allVarsExcept_finIdxOf?_none_if_diff_path_conds (by simp [Ne.symm h₃])]
+          simp [hchans₃_no_var, h₃]
       else
-        compileExpr.allVarsExcept χ ec.definedVars [cond] rightConds)
-      = compileExpr.allVarsExcept χ ec.definedVars [cond]
-        ((condBool, ChanName.var cond ec.pathConds) :: ec.pathConds)
-    := by
-      simp only [← hleftConds, ← hrightConds, ← hcondName]
-      cases condBool <;> simp
-    rw [this] at hsteps₂; clear this
-    apply step_plus_eq _ _ _ _ hsteps₂
-    simp [hpc₁]
-    funext name
-    simp only [SimR.varsToChans]
-    cases name with
-    | var v pathConds =>
-      simp
-      if h₁ : v = cond then
-        rw [allVarsExcept_finIdxOf?_none_if_removed (by simp [h₁])]
-        simp [h₁, VarMap.getVar, VarMap.removeVar, hchans₃, hchans₂, hpc₁, hchans₁,
-          hlive_vars, SimR.varsToChans, ← hcondName,
-          List.finIdxOf?, List.findFinIdx?, List.findFinIdx?.go]
-        intros _ h₂ h₃
-        exact False.elim (h₂ h₃)
-      else
-        if h₂ : v ∈ ec.definedVars then
-          if h₃ : pathConds = (condBool, ChanName.var cond ec.pathConds) :: ec.pathConds then
-            have ⟨i, h₄⟩ := allVarsExcept_finIdxOf?_some (removedVars := [cond])
-              h₂ (by simp [h₁]) h₃
-            simp [h₄]
-            simp [compileExpr.allVarsExcept] at h₄
-            simp [List.toVector] at h₄
-            simp [h₄.1.2, Ne.symm h₁, VarMap.getVar, VarMap.removeVar]
-            have ⟨_, h₅⟩ := (hdefined_vars v).mp h₂
-            simp only [VarMap.getVar] at h₅
-            have := List.forall₂_iff_get.mp hall_vals
-            have := this.2 i (by simp) (by simp)
-            simp [List.toVector, VarMap.getVar, compileExpr.allVarsExcept, h₄.1.1] at this
-            simp [this]
-          else
-            rw [allVarsExcept_finIdxOf?_none_if_diff_path_conds (by simp [Ne.symm h₃])]
-            simp [hchans₃_no_var, h₃]
-        else
-          rw [allVarsExcept_finIdxOf?_none_if_not_defined (by simp [h₂])]
-          simp [hchans₃_no_var]
-          split
-          · rename_i h₃
-            simp [VarMap.getVar, VarMap.removeVar] at h₃
-            have := (hdefined_vars v).mpr ⟨_, h₃.2⟩
-            simp [h₂ this]
-          · simp
-    | merge_cond name =>
-      simp [hchans₃, hchans₂, hpc₁, hchans₁,
-        compileExpr.allVarsExcept, List.finIdxOf?, List.findFinIdx?, List.findFinIdx?.go]
-      if h₁ : condName = name then
-        simp [h₁]
-        simp [hcondName, Eq.symm h₁]
-        have := instInterp.unique_toBool_fromBool _ _ hcondBool
-        if h₂ : condBool then
-          simp [h₂] at this ⊢
-          exact this
-        else
-          simp [h₂] at this ⊢
-          split
-          · rename_i h
-            simp only [← hcondName] at h
-            have := hpath_conds_order _ _ _ h
-            omega
-          · simp [this]
-      else
-        cases condBool
-        all_goals
-        simp [h₁]
-        simp [hcondName, Ne.symm h₁]
-        simp [← hcondName, hlive_vars, SimR.varsToChans]
-    | switch_cond name =>
+        rw [allVarsExcept_finIdxOf?_none_if_not_defined (by simp [h₂])]
+        simp [hchans₃_no_var]
+        split
+        · rename_i h₃
+          simp [VarMap.getVar, VarMap.removeVar] at h₃
+          have := hsim.get_var_to_defined_vars ⟨_, h₃.2⟩
+          simp [h₂ this]
+        · simp
+  | merge_cond name =>
+    simp [hchans₃, hchans₂, hpc₁, hchans₁,
+      compileExpr.allVarsExcept, List.finIdxOf?, List.findFinIdx?, List.findFinIdx?.go]
+    if h₁ : condName = name then
+      simp [h₁]
+      simp [hcond_name, Eq.symm h₁]
+      have := instInterp.unique_toBool_fromBool _ _ hcondBool
+      simp [this, ← hcond_name, hsim.path_conds_acyclic]
+      split <;> (rename_i h₂; simp [h₂])
+    else
       cases condBool
       all_goals
-        simp [compileExpr.allVarsExcept, hchans₃, hchans₂, hpc₁, hchans₁]
-        intro h
-        simp [Ne.symm h, hlive_vars, SimR.varsToChans,
-          List.finIdxOf?, List.findFinIdx?, List.findFinIdx?.go]
-    | _ =>
-      cases condBool
-      all_goals
-        simp [compileExpr.allVarsExcept, hchans₃, hchans₂, hchans₁, hpc₁]
-        try rw [(Vector.finIdxOf?_eq_none_iff).mpr _]
-        simp [← hcondName, hlive_vars, hbr, SimR.varsToChans,
-          List.finIdxOf?, List.findFinIdx?, List.findFinIdx?.go]
+      simp [h₁]
+      simp [hcond_name, Ne.symm h₁]
+      simp [← hcond_name, hsim.vars_to_chans, varsToChans]
+  | switch_cond name =>
+    cases condBool
+    all_goals
+      simp [compileExpr.allVarsExcept, hchans₃, hchans₂, hpc₁, hchans₁]
+      intro h
+      simp [Ne.symm h, hsim.vars_to_chans, varsToChans,
+        List.finIdxOf?, List.findFinIdx?, List.findFinIdx?.go]
+  | _ =>
+    cases condBool
+    all_goals
+      simp [compileExpr.allVarsExcept, hchans₃, hchans₂, hchans₁, hpc₁]
+      try rw [(Vector.finIdxOf?_eq_none_iff).mpr _]
+      simp [← hcond_name, hsim.vars_to_chans, hbr, varsToChans,
+        List.finIdxOf?, List.findFinIdx?, List.findFinIdx?.go]
 
 theorem sim_step_br
   [Arity Op] [DecidableEq χ] [instInterp : Interp Op V S]
   {cond left right}
   {ec ec' : Seq.Config Op χ V S m n}
   {pc : Dataflow.Config Op (ChanName χ) V S m n}
-  (hnz : m > 0 ∧ n > 0)
-  (hsim : SimR _ _ _ _ hnz ec pc)
+  {hnz : m > 0 ∧ n > 0}
+  (hsim : SimRel hnz ec pc)
   (hstep : Config.Step Op χ V S ec ec')
   (hbr : ec.expr = .cont (.br cond left right)) :
   ∃ pc',
     Config.StepPlus Op (ChanName χ) V S pc pc' ∧
-    SimR _ _ _ _ hnz ec' pc' := by
-  have ⟨
-    heq_state,
-    hlive_vars,
-    hdefined_vars_no_dup,
-    hdefined_vars,
-    hpath_conds_order,
-    hpath_conds_nodup,
-    hmerges,
-    hwf_fn,
-    ⟨
-      rest, carryInLoop, ctxLeft, ctxCurrent, ctxRight,
-      hatoms,
-      hcomp_fn,
-      hrest,
-      hret,
-      hcont,
-    ⟩,
-  ⟩ := hsim
-  have ⟨hcarryInLoop, hwf_expr, hcurrent⟩ := hcont _ hbr
-  simp only [compileExpr] at hcurrent
-  have hsteps := sim_step_br_chans hnz hsim hstep hbr
+    SimRel hnz ec' pc' := by
+  have hsteps := sim_step_br_exec_dataflow hsim hstep hbr
   replace ⟨pc', hpc', hsteps⟩ := exists_eq_left.mpr hsteps
   -- Deduce some facts from `hstep`
+  have ⟨
+    rest, carryInLoop, ctxLeft, ctxCurrent, ctxRight,
+    hatoms, hcomp_fn, hrest, hret, hcont,
+  ⟩ := hsim.has_compiled_procs
+  have ⟨hcarryInLoop, hwf_expr, hcurrent⟩ := hcont _ hbr
   cases hstep with
   | step_ret hexpr | step_tail hexpr | step_op hexpr =>
     simp [hbr] at hexpr
@@ -304,23 +262,18 @@ theorem sim_step_br
     · exact hsteps
     · simp only [hpc']
       and_intros
-      · simp [heq_state]
+      · simp [hsim.eq_state]
       · simp
-      · exact List.Nodup.filter _ hdefined_vars_no_dup
-      · simp; grind [VarMap.getVar, VarMap.removeVar]
-      · simp; grind [SimR.OrderedPathConds]
-      · simp; grind [SimR.OrderedPathConds]
-      · simp; grind [compileExpr.varName]
-      · simp only [hmerges]
-      · exact hwf_fn.1
-      · exact hwf_fn.2
+      · exact List.Nodup.filter _ hsim.defined_vars_nodup
+      · simp; grind [VarMap.removeVar, VarMap.getVar]
+      · simp; grind
+      · simp; grind
       · simp
-        grind only [compileExpr.varName,
-          List.length_cons, =_ List.cons_append, usr List.length_filter_le,
-          = List.removeAll_nil, = List.removeAll_cons, = List.append_assoc,
-          =_ List.countP_eq_length_filter, = List.nodup_iff_count, List.length_nil, List.nil_append,
-          List.append_nil, = List.cons_append, List.Pairwise.map, = List.nodup_iff_pairwise_ne,
-          =_ List.append_assoc, = List.pairwise_map, = List.countP_eq_length_filter',
-          → List.eq_nil_of_append_eq_nil, List.size_toArray, → List.eq_nil_of_map_eq_nil, cases Or]
+        grind [compileExpr, compileExpr.varName, compileExpr.brMerge]
+      · simp only [hsim.has_merges]
+      · exact hsim.wf_fn.1
+      · exact hsim.wf_fn.2
+      · simp [HasCompiledProcs]
+        grind [compileExpr, compileExpr.varName]
 
 end Wavelet.Simulation.Br
