Wavelet/Simulation/Invariants.lean
@@ -1,0 +1,164 @@
+import Mathlib.Logic.Relation
+
+import Wavelet.Op
+import Wavelet.Seq
+import Wavelet.Dataflow
+import Wavelet.Compile
+
+/-! Simulation invariants for the compilation from `Seq` to `Dataflow`. -/
+
+namespace Wavelet.Simulation.Invariants
+
+open Op Seq Dataflow Compile
+
+def varsToChans
+  [Arity Op] [instInterp : Interp Op V S]
+  (ec : Seq.Config Op χ V S m n) : ChanMap (ChanName χ) V :=
+  λ name =>
+    match name with
+    | .var v pathConds =>
+      if pathConds = ec.pathConds then
+        if let some val := ec.vars.getVar _ _ v then
+          [val]
+        else []
+      else []
+    | .merge_cond v =>
+      if (true, v) ∈ ec.pathConds then
+        [instInterp.fromBool true]
+      else if (false, v) ∈ ec.pathConds then
+        [instInterp.fromBool false]
+      else []
+    | .final_dest i =>
+      -- Corresponding final return values
+      if let .ret vals := ec.expr then
+        if _ : i < n then [vals[i]]
+        else []
+      else []
+    | _ => []
+
+@[grind]
+def HasMerges
+  [Arity Op]
+  (m n : Nat)
+  (atoms : AtomicProcs Op (ChanName χ) V) :
+  List (Bool × ChanName χ) → Prop
+  | [] => True
+  | (_, chan) :: rest =>
+    (compileExpr.brMerge _ _ _ m n chan rest ∈ atoms) ∧
+    HasMerges m n atoms rest
+
+@[grind]
+def OrderedPathConds (pathConds : List (Bool × ChanName χ)) : Prop :=
+  (∀ b var pathConds', (b, ChanName.var var pathConds') ∈ pathConds →
+    pathConds'.length < pathConds.length)
+
+/-- Invariants that the processes should correspond
+to the compiled expressions/fns. -/
+@[grind]
+def HasCompiledProcs
+  [Arity Op] [Interp Op V S] [DecidableEq χ]
+  (hnz : m > 0 ∧ n > 0)
+  (ec : Seq.Config Op χ V S m n)
+  (pc : Dataflow.Config Op (ChanName χ) V S m n) : Prop :=
+  ∃ (rest : AtomicProcs Op (ChanName χ) V)
+    (carryInLoop : Bool)
+    (ctxLeft ctxCurrent ctxRight : AtomicProcs Op (ChanName χ) V),
+    pc.proc.atoms = compileFn.initCarry _ _ _ ec.fn carryInLoop :: rest ∧
+    (compileFn Op χ V S hnz ec.fn).atoms = compileFn.initCarry _ _ _ ec.fn false :: rest ∧
+    rest = ctxLeft ++ ctxCurrent ++ ctxRight ∧
+    (∀ vals, ec.expr = .ret vals → ¬ carryInLoop ∧
+      ctxCurrent = [] ∧
+      ctxRight = [] ∧
+      ec.definedVars = [] ∧
+      ec.pathConds = []) ∧
+    (∀ expr, ec.expr = .cont expr → carryInLoop ∧
+      expr.WellFormed _ _ ec.definedVars ∧
+      compileExpr Op χ V S hnz ec.definedVars ec.pathConds expr = ctxCurrent)
+
+@[grind]
+def SimRel
+  [Arity Op] [Interp Op V S] [DecidableEq χ]
+  (hnz : m > 0 ∧ n > 0)
+  (ec : Seq.Config Op χ V S m n)
+  (pc : Dataflow.Config Op (ChanName χ) V S m n) : Prop :=
+  ec.state = pc.state ∧
+  -- Some invariants about the correspondence between variables and channels
+  pc.chans = varsToChans ec ∧
+  ec.definedVars.Nodup ∧
+  (∀ var, var ∈ ec.definedVars ↔ ∃ val, ec.vars.getVar _ _ var = some val) ∧
+  OrderedPathConds ec.pathConds ∧
+  -- No path condition are pushed twice
+  (ec.pathConds.map Prod.snd).Nodup ∧
+  -- Some invariants about the "shape" of the processes
+  HasMerges m n pc.proc.atoms ec.pathConds ∧
+  ec.fn.WellFormed ∧
+  HasCompiledProcs hnz ec pc
+
+/-! Utility functions to extract facts from the simulation relation. -/
+section Utilities
+
+variable {Op χ V S}
+variable [Arity Op] [Interp Op V S] [DecidableEq χ]
+variable {ec : Seq.Config Op χ V S m n}
+variable {pc : Dataflow.Config Op (ChanName χ) V S m n}
+variable {hnz : m > 0 ∧ n > 0}
+variable (hsim : SimRel hnz ec pc)
+
+def SimRel.eq_state : ec.state = pc.state := hsim.1
+
+def SimRel.vars_to_chans : pc.chans = varsToChans ec := hsim.2.1
+
+def SimRel.wf_fn : ec.fn.WellFormed := by
+  have ⟨_, _, _, _, _, _, _, h, _⟩ := hsim
+  exact h
+
+def SimRel.defined_vars_nodup : ec.definedVars.Nodup := hsim.2.2.1
+
+def SimRel.defined_vars_to_get_var :
+  var ∈ ec.definedVars → ∃ val, ec.vars.getVar _ _ var = some val := by
+  have ⟨_, _, _, h, _⟩ := hsim
+  apply (h var).mp
+
+def SimRel.get_var_to_defined_vars :
+  (∃ val, ec.vars.getVar _ _ var = some val) → var ∈ ec.definedVars := by
+  have ⟨_, _, _, h, _⟩ := hsim
+  apply (h var).mpr
+
+def SimRel.defined_vars_iff_get_var
+  : var ∈ ec.definedVars ↔ ∃ val, ec.vars.getVar _ _ var = some val := by
+  have ⟨_, _, _, h, _⟩ := hsim
+  exact h var
+
+def SimRel.path_conds_nodup : (ec.pathConds.map Prod.snd).Nodup := by
+  have ⟨_, _, _, _, _, h, _⟩ := hsim
+  exact h
+
+def SimRel.path_conds_acyclic : (b, .var v ec.pathConds) ∉ ec.pathConds := by
+  intros h'
+  have ⟨_, _, _, _, h, _⟩ := hsim
+  have := h _ _ _ h'
+  simp at this
+
+def SimRel.has_merges : HasMerges m n pc.proc.atoms ec.pathConds := by
+  have ⟨_, _, _, _, _, _, h, _⟩ := hsim
+  exact h
+
+def SimRel.has_compiled_procs : HasCompiledProcs hnz ec pc := by
+  have ⟨_, _, _, _, _, _, _, _, h⟩ := hsim
+  exact h
+
+def SimRel.final_config_empty_defined_vars
+  (h : ec.expr = .ret vals) : ec.definedVars = [] := by
+  have ⟨_, _, _, _, _, _, _, _, hret, _⟩ := hsim.has_compiled_procs
+  have ⟨_, _, _, h, _⟩ := hret _ h
+  exact h
+
+def SimRel.final_config_empty_path_conds
+  (h : ec.expr = .ret vals) : ec.pathConds = [] := by
+  have ⟨_, _, _, _, _, _, _, _, hret, _⟩ := hsim.has_compiled_procs
+  have ⟨_, _, _, _, h⟩ := hret _ h
+  exact h
+
+end Utilities
+
+end Wavelet.Simulation.Invariants
